work on MapDefault

theories/Events/MapDefaultFacts.v
@@ -38,12 +38,12 @@ Section MapFacts.
   Context {map : Type}.
   Context {M : Map K V map}.
 
-  Global Instance eq_map_refl {d} : Reflexive (eq_map d).
+  Global Instance eq_map_refl {d} : Reflexive (@eq_map _ _ _ _ d).
   Proof.
     red. intros. unfold eq_map. tauto.
   Qed.    
 
-  Global Instance eq_map_sym {d} : Symmetric (eq_map d).
+  Global Instance eq_map_sym {d} : Symmetric (@eq_map _ _ _ _ d).
   Proof.
     repeat intro.
     unfold eq_map in H.
@@ -51,7 +51,7 @@ Section MapFacts.
     reflexivity.
   Qed.
 
-  Global Instance eq_map_trans {d} : Transitive (eq_map d).
+  Global Instance eq_map_trans {d} : Transitive (@eq_map _ _ _ _ d).
   Proof.
     repeat intro. 
     unfold eq_map in *.
@@ -65,12 +65,12 @@ Section MapFacts.
 
   Definition map_default_eq d {E} 
     : (stateT map (itree E) R1) -> (stateT map (itree E) R2) -> Prop :=
-    fun t1 t2 => forall s1 s2, eq_map d s1 s2 -> eutt (prod_rel (eq_map d) RR) (t1 s1) (t2 s2).
+    fun t1 t2 => forall s1 s2, (@eq_map _ _ _ _ d) s1 s2 -> eutt (prod_rel (@eq_map _ _ _ _ d) RR) (t1 s1) (t2 s2).
 
   End Relations.
 
   Lemma eq_map_add:
-    forall (d : V) (s1 s2 : map) (k : K) (v : V), eq_map d s1 s2 -> eq_map d (add k v s1) (add k v s2).
+    forall (d : V) (s1 s2 : map) (k : K) (v : V), (@eq_map _ _ _ _ d) s1 s2 -> (@eq_map _ _ _ _ d) (add k v s1) (add k v s2).
   Proof.
     intros d s1 s2 k v H.
     unfold eq_map in *.
@@ -79,16 +79,16 @@ Section MapFacts.
   Admitted.
 
   Lemma eq_map_remove:
-    forall (d : V) (s1 s2 : map) (k : K), eq_map d s1 s2 -> eq_map d (remove k s1) (remove k s2).
+    forall (d : V) (s1 s2 : map) (k : K), (@eq_map _ _ _ _ d) s1 s2 -> (@eq_map _ _ _ _ d) (remove k s1) (remove k s2).
   Proof.
     intros d s1 s2 k H.
   Admitted.
 
   
   Lemma handle_map_eq : 
-    forall d E X (s1 s2 : map) (m : mapE d X),
-      eq_map d s1 s2 ->
-      eq_itree (prod_rel (eq_map d) eq) (handle_map m s1) ((handle_map m s2) : itree E (map * X)).
+    forall d E X (s1 s2 : map) (m : mapE K d X),
+      (@eq_map _ _ _ _ d) s1 s2 ->
+      eutt (prod_rel (@eq_map _ _ _ _ d) eq) (handle_map m s1) ((handle_map m s2) : itree E (map * X)).
   Proof.
     intros.
     destruct m; cbn; red; apply eqit_Ret; constructor; auto.
@@ -96,9 +96,20 @@ Section MapFacts.
     - apply eq_map_remove. assumption.
   Qed.
 
+
+  Global Instance Proper_handle_map {E R}  d :
+    Proper (eq ==> map_default_eq eq d) (@handle_map _ _ _ _ E d R).
+  Proof.
+    repeat intro.
+    subst.
+    apply handle_map_eq.
+    assumption.
+  Qed.
+    
+  
   (* This lemma states that the operations provided by [handle_map] respect
      the equivalence on the underlying map interface *)
-  Lemma run_map_id d {E X} (t : itree (mapE d +' E) X) :
+  Lemma run_map_id d {E X} (t : itree (mapE K d +' E) X) :
     map_default_eq eq d (run_map t) (run_map t).
   Proof.
     unfold map_default_eq, run_map; intros.
@@ -121,7 +132,40 @@ Section MapFacts.
         inversion H. subst.
         gbase. apply CH. assumption.
   Qed.
-
-
+ 
+  Global Instance run_map_proper {R E d} {RR : R -> R -> Prop} :
+    Proper ((eutt RR) ==> (@map_default_eq _ _ RR d E)) (@run_map _ _ _ _ E d R).
+  Proof.
+    unfold map_default_eq, run_map.
+    repeat intro.
+    revert x y H s1 s2 H0.
+    einit.
+    ecofix CH.
+    intros.
+    rewrite! unfold_interp_state. 
+    punfold H0. red in H0.
+    revert s1 s2 H1.
+    induction H0; intros; subst; simpl; pclearbot.
+    - eret.
+    - etau.
+    - etau.
+      ebind.
+      apply pbc_intro_h with (RU := prod_rel (@eq_map _ _ _ _ d) eq).
+      { (* SAZ: I must be missing some lemma that should solve this case *)
+        unfold case_. unfold Case_sum1, case_sum1.
+        destruct e. apply handle_map_eq. assumption.
+        unfold pure_state.
+        pstep. econstructor. intros. constructor. pfold. econstructor. constructor; auto.
+      } 
+      intros.
+      inversion H. subst.
+      simpl.
+      ebase.
+    - rewrite tau_eutt, unfold_interp_state.
+      eauto.
+    - rewrite tau_eutt, unfold_interp_state.
+      eauto.
+  Qed.
+    
   
 End MapFacts.
